execution/theories/CongressTests.v
@@ -1,0 +1,117 @@
+From ConCert Require Import Generators Blockchain LocalBlockchain Congress.
+From ConCert Require Import Serializable.
+From ConCert Require Import BoundedN ChainedList.
+Require Import ZArith Strings.Ascii Strings.String.
+
+From QuickChick Require Import QuickChick. Import QcNotation.
+From ExtLib.Structures Require Import Functor Applicative.
+Require Export ExtLib.Structures.Monads.
+Export MonadNotation. Open Scope monad_scope.
+From Coq Require Import List.
+From Coq Require Import Strings.BinaryString.
+From Coq Require Import Morphisms.
+From Coq Require Import Program.Basics.
+Import ListNotations.
+Notation "f 'o' g" := (compose f g) (at level 50).
+
+(* Generators for the types defined in the Congress contract *)
+
+Let BaseTypes := LocalChainBase AddrSize.
+Example ca : @CongressAction BaseTypes := cact_transfer zero_address 0%Z.
+Open Scope string_scope.
+
+Instance showRules : Show Rules :=
+  {|
+    show r := 
+      "Rules{"
+      ++ "min_vote_count_permille: " ++ show (min_vote_count_permille r) ++ sep
+      ++ "margin_needed_permille: " ++ show (margin_needed_permille r) ++ sep
+      ++ "debating_period_in_blocks: " ++ show (debating_period_in_blocks r) 
+      ++ "}"
+  |}.
+
+Instance showCongressAction `{Show SerializedValue} : Show CongressAction :=
+  {|
+    show ca :=
+      match ca with
+      | cact_transfer to amount => "(transfer: " ++ show to ++ sep ++ show amount ++ ")"
+      | cact_call to amount msg => "(call: " ++ show to ++ sep ++ show amount ++ sep ++ show msg ++ ")" 
+      end
+  |}.
+
+Instance showProposal : Show Proposal :=
+  {|
+    show p :=
+      "Proposal{"
+      ++ "actions: " ++ show (actions p)
+      ++ "votes: " ++ "..." (*show (votes p)*)
+      ++ "vote_result: " ++ show (vote_result p) 
+      ++ "proposed_in: " ++ show (proposed_in p) 
+      ++ "}"
+  |}.
+
+Instance showSetup : Show Setup :=
+  {|
+    show := show o setup_rules
+  |}.
+
+Definition string_of_Msg (m : Msg) : string :=
+  match m with
+    | transfer_ownership addr => "(transfer_ownership " ++  show addr ++ ")"
+    | change_rules rules => "(change_rules " ++ show rules ++ ")"
+    | add_member addr => "(add_member " ++ show addr ++ ")"
+    | remove_member addr => "(remove_member " ++ show addr ++ ")"
+    | create_proposal actions => "(create_proposal " ++ show actions ++ ")"
+    | vote_for_proposal proposalId => "(vote_for_proposal " ++ show proposalId ++ ")"
+    | vote_against_proposal proposalId => "(vote_against_proposal " ++ show proposalId ++ ")"
+    | retract_vote proposalId => "(retract_vote " ++ show proposalId ++ ")"
+    | finish_proposal proposalId => "(finish_proposal " ++ show proposalId ++ ")"
+  end.
+
+Instance showMsg : Show Msg :=
+{|
+  show := string_of_Msg
+|}.
+
+Close Scope string_scope.
+
+Definition gRulesSized (n : nat) : G Rules :=
+  vote_count <- arbitrarySized n ;;
+  margin <- liftM Z.of_nat (gIntervalNat n (2 * n)) ;;
+  liftM (build_rules vote_count margin) arbitrary.  
+
+Instance genRulesSized : GenSized Rules :=
+  {|
+    arbitrarySized := gRulesSized
+  |}.
+
+
+Definition gCongressAction {ctx : ChainContext BaseTypes}
+                           (gMsg : G SerializedValue) 
+                           : G CongressAction :=
+  let gAddr := (gInvalidContractAddr BaseTypes ctx) in
+  freq [
+    (1, liftM2 cact_transfer gAddr arbitrary);
+    (1, liftM3 cact_call gAddr arbitrary gMsg)
+  ].
+
+Fixpoint gMsgSized {ctx : ChainContext BaseTypes} (n : nat) : G Msg :=
+  let nonrec_gens := [
+      (1, liftM transfer_ownership (gInvalidContractAddr _ ctx)) ;
+      (1, liftM change_rules arbitrary) ;
+      (1, liftM add_member (gInvalidContractAddr _ ctx)) ;
+      (1, liftM remove_member (gInvalidContractAddr _ ctx)) ;
+      (1, liftM vote_for_proposal arbitrary) ;
+      (1, liftM vote_against_proposal arbitrary) ;
+      (1, liftM retract_vote arbitrary) ;
+      (1, liftM finish_proposal arbitrary)
+    ] in 
+  let default := liftM transfer_ownership (gInvalidContractAddr _ ctx) in
+  match n with
+    | 0 => (freq_ default nonrec_gens)
+    | S n' =>
+    let rec_gens := 
+      (1, liftM create_proposal (listOf (@gCongressAction ctx (liftM serialize (@gMsgSized ctx n')))))
+      :: nonrec_gens in
+    freq_ default rec_gens
+  end.
